wip

IterTree/Basic.lean
@@ -10,10 +10,10 @@ branching tree, which give rise to the different possible traces.
 The type of an iTree is parametrized by two types:
  - R, the type of values returned by the computation
  - E, the possible events raised by the computation before it concludes. Data may be
-   requested by the computation before it can resume, and the event is allowed to 
+   requested by the computation before it can resume, and the event is allowed to
    depend on the type of this data.
 
-We would write this as 
+We would write this as
 
     coinductive iTree (E : Type → Type) (R : Type) where
     | ret : R → iTree E R
@@ -77,41 +77,41 @@ the iTrees we're comparing through our stripping function first.
 
 -/
 
-def stripTau : iTree E R → iTree E R 
+def stripTau : iTree E R → iTree E R
 | .ret v => .ret v
 | .tau it => it.stripTau
 | .vis ev k => .vis ev (fun it => (k it).stripTau)
 
-theorem eqUpToTau_of_stripTau_eq_stripTau {it₁ it₂ : iTree E R} : (it₁.stripTau = it₂.stripTau) → it₁.eqUpToTau it₂ := by 
+theorem eqUpToTau_of_stripTau_eq_stripTau {it₁ it₂ : iTree E R} : (it₁.stripTau = it₂.stripTau) → it₁.eqUpToTau it₂ := by
   intros hyp
   induction it₁ generalizing it₂ with
   | ret v₁ =>
-    induction it₂ with 
-    | ret v₂ => 
+    induction it₂ with
+    | ret v₂ =>
       grind [eqUpToTau, stripTau]
-    | tau it₂ => 
+    | tau it₂ =>
       grind [stripTau, eqUpToTau]
-    | vis ev₂ k₂ => 
+    | vis ev₂ k₂ =>
       simp [stripTau] at hyp
   | tau it₁ IH =>
     grind [stripTau, eqUpToTau]
   | vis ev₁ k₁ IH₁ =>
-    induction it₂ with 
-    | ret v₂ => 
+    induction it₂ with
+    | ret v₂ =>
       grind [eqUpToTau, stripTau]
-    | tau it₂ => 
+    | tau it₂ =>
       grind [stripTau, eqUpToTau]
-    | vis ev₂ k₂ IH₂ => 
+    | vis ev₂ k₂ IH₂ =>
       simp [stripTau] at hyp
       obtain ⟨rfl, rfl, hyp⟩ :=  hyp
       simp only [heq_eq_eq] at hyp
       replace hyp := fun a => congrFun hyp a
       constructor
-      intros a 
+      intros a
       apply IH₁
       grind
 
-theorem eqUpToTau_iff_stripTau_eq_stripTau {it₁ it₂ : iTree E R} : it₁.eqUpToTau it₂ ↔ (it₁.stripTau = it₂.stripTau) := by 
+theorem eqUpToTau_iff_stripTau_eq_stripTau {it₁ it₂ : iTree E R} : it₁.eqUpToTau it₂ ↔ (it₁.stripTau = it₂.stripTau) := by
   constructor <;> intros hyp
   · induction hyp <;> grind [stripTau]
   · apply eqUpToTau_of_stripTau_eq_stripTau hyp
@@ -121,19 +121,19 @@ end iTree
 end Finite
 
 
-/- 
+/-
 
-Therefore, we look to give a different presentation of iTrees, which does not have this problem, but also 
+Therefore, we look to give a different presentation of iTrees, which does not have this problem, but also
 allows definining the same operations as the finite case.
 
--/ 
+-/
 
 namespace StateMachine
 
-/- 
+/-
 
 The first attempt I want to try is to give an encoding in terms of a state machine. Basically, we have a
-"current state" and a "step function" which tells us to what state to go next. 
+"current state" and a "step function" which tells us to what state to go next.
 
 The issue with this representation is that a single, fixed state is not enough to express all we want out
 of iTrees (Is this actually true?).
@@ -151,7 +151,7 @@ inductive Obs (E : Type q → Type r) (R : Type v) (K : Type k) where
 | tau : K → Obs E R K
 | vis {A : Type q} : E A → (A → K) → Obs E R K
 
-def Obs.mapState (f : α → β) : Obs E R α → Obs E R β 
+def Obs.mapState (f : α → β) : Obs E R α → Obs E R β
 | .ret v => .ret v
 | .tau st => .tau <| f st
 | .vis ev k => .vis ev (fun x => f (k x))
@@ -174,7 +174,7 @@ structure iTree (E : Type q → Type r) (R : Type v) where
   -- Why not have it give observations on just `State`?
   -- I think it's not possible, because we must be able to change
   -- the state type at some point in the execution.
-  -- 
+  --
   -- However, how do you define the infinitely looping
   -- computation with `State → Obs E R (iTree E R)`?
   -- You can't, you'd need to reference back to the think you're
@@ -185,17 +185,17 @@ structure iTree (E : Type q → Type r) (R : Type v) where
   -- It also can't be `State → Obs E R State` because one should
   -- be able to encode that the state changes from one computation
   -- to another. Or can't it?
-  -- 
-  -- The issue with doing this encoding is that one must fix the 
+  --
+  -- The issue with doing this encoding is that one must fix the
   -- type of the state of the final computation, but it's not
   -- trivial to define. For instance, one would like to say that
-  -- when doing a `bind` with `f`, the state will originally be 
+  -- when doing a `bind` with `f`, the state will originally be
   -- that of the interaction tree being executed, until it gives
-  -- a value `a`, at which point one switches to the state of the 
-  -- `iTree` resulting from applying `f` to `a`. However, this 
+  -- a value `a`, at which point one switches to the state of the
+  -- `iTree` resulting from applying `f` to `a`. However, this
   -- cannot be expressed directly as a type.
-  -- One could, however, express this as an invariant of the 
-  -- structure, which leads us back to the `IsPlausibleStep` of 
+  -- One could, however, express this as an invariant of the
+  -- structure, which leads us back to the `IsPlausibleStep` of
   -- `Std.Iter`.
 /-
 
@@ -214,21 +214,19 @@ def loop.{s} : iTree E R where
   curr := .unit
   step _ := .tau .unit
 
-set_option pp.universes true in #print loop
-
 instance : Inhabited (iTree E R) := ⟨loop⟩
-  
-def unfold (it : iTree E R) : Obs E R (iTree E R) := 
-  match it.step it.curr with 
+
+def unfold (it : iTree E R) : Obs E R (iTree E R) :=
+  match it.step it.curr with
   | .ret v => .ret v
   | .tau next => .tau {it with curr := next}
   | .vis ev k => .vis ev (fun x => {it with curr := (k x)})
 
 theorem unfold_cases (it : iTree E R) :
     (∃ v, it.unfold = .ret v) ∨
-    (∃ (α : Type _) (ev : E α) (k : α → iTree E R), it.unfold = .vis ev k) ∨ 
-    (∃ it', it.unfold = .tau it') := 
-  match it.unfold with 
+    (∃ (α : Type _) (ev : E α) (k : α → iTree E R), it.unfold = .vis ev k) ∨
+    (∃ it', it.unfold = .tau it') :=
+  match it.unfold with
   | .ret v => .inl ⟨v, rfl⟩
   | .vis (A := α) ev k => .inr <| .inl ⟨α, ev, k, rfl⟩
   | .tau next => .inr <| .inr ⟨next, rfl⟩
@@ -238,53 +236,57 @@ theorem unfold_cases (it : iTree E R) :
 -- Maybe this can be defined later, once we have equality over unfoldings.
 /- def recUnfold {motive : iTree E R → Prop} -/
 /-   (onRet : (v : R) → motive (.ret v)) -/
-/-   (onTau : (it iTree E R → -/ 
+/-   (onTau : (it iTree E R → -/
 
-def ret (r : R) : iTree E R where
-  curr : Unit  := ()
+def ret.{s} (r : R) : iTree E R where
+  curr : PUnit.{s+1}  := .unit
   step _ := .ret r
 
-set_option pp.universes true in #print ret
-
-def vis {α} (ev : E α) (k : α → iTree E R) : iTree E R where
-  curr : Unit ⊕ (a : α) × (k a ).State := .inl ()
-  step 
-  | .inl () => .vis ev (fun a => .inr <| ⟨a, (k a).curr⟩)
-  | .inr ⟨a, s⟩ => (k a).step s |>.mapState (.inr ⟨a, ·⟩)
-
-def tau (it : iTree E R) : iTree E R where
-  -- We basically generate an artificial prior element in the state.
-  curr : Unit ⊕ it.State  := .inl ()
+def vis.{s} {α : Type q} (ev : E α) (k : α → iTree.{_,_,_,s} E R) : iTree E R where
+  curr : PUnit.{max q s +1} ⊕ (a : α) × (k a ).State := .inl .unit
   step
-  | .inl () => .tau <| .inr <| it.curr
+  | .inl .unit => .vis ev (fun a => .inr <| ⟨a, (k a).curr⟩)
+  | .inr ⟨a, s⟩ => (k a).step s |>.mapState (.inr ⟨a, ·⟩)
+  -- TODO: I could probably generalize this structure of
+  -- "stay in inl until something, then inr always", and
+  -- prove some generic lemmas about it, to reduce the proof
+  -- burden.
+  -- Would also be cool to state that "once a is chosen, it
+  -- doesn't change"
+
+def tau.{s} (it : iTree.{_,_,_,s} E R) : iTree E R where
+  -- We basically generate an artificial prior element in the state.
+  curr : PUnit.{s+1} ⊕ it.State  := .inl .unit
+  step
+  | .inl .unit => .tau <| .inr <| it.curr
   | .inr s => it.step s |>.mapState (.inr)
 
 end iTree
 
-def Obs.toITree : Obs E R (iTree E R) → iTree E R 
+def Obs.toITree : Obs E R (iTree E R) → iTree E R
 | .tau it => iTree.tau it
 | .vis ev k => iTree.vis ev k
 | .ret v => iTree.ret v
-  
+
 
 namespace iTree
 
 
 /--
   After the computation of the interaction tree `it`, we simply continue with the
-  computation given by `f`. We encode the information of the continuation in the 
+  computation given by `f`. We encode the information of the continuation in the
   closure, to dodge problems with termination.
 -/
 def bindLeft {α β} (f : α → iTree E β)(it : iTree E α) : iTree E β where
     curr : it.State ⊕ (a : α) × (f a).State := .inl it.curr
-    step st := 
-      match st with 
+    step st :=
+      match st with
       | .inl curr =>
-        it.step curr 
-        |>.mapState .inl 
+        it.step curr
+        |>.mapState .inl
         |>.bindVal (fun a => .tau <| .inr ⟨a, (f a).curr⟩)
       | .inr ⟨a, st⟩ =>
-        (f a).step st 
+        (f a).step st
         |>.mapState (.inr ⟨a, ·⟩)
 
 instance : Bind (iTree E) := ⟨(·.bindLeft ·)⟩
@@ -317,7 +319,7 @@ to care about the internal state of your iTree.
 Then there is an "extensional" equality, or "observational" equality, which
 cares only for the observable behaviour of iTrees. In particular, it does
 away with the details of the internal state, and only cares for the `Obs`
-produced by the `step` function. 
+produced by the `step` function.
 
 However, this is not the best notion of equality either. We also have
 equivalences between iTrees which are equivalent in their observations if
@@ -328,12 +330,12 @@ the concept of what a "computation" is.
 
 namespace WrongEq
 
-/-- 
+/--
   This is the wrong notion of equality!
 
   It allows one to identify `fun _ => .ret 0` with `.skip`!
 -/
-def eq {α} (it₁ it₂ : iTree E α) : Prop := 
+def eq {α} (it₁ it₂ : iTree E α) : Prop :=
   match it₁.unfold, it₂.unfold with
   | .ret v₁, .ret v₂ => v₁ = v₂
   | @Obs.vis _ _ _ A₁ ev₁ k₁, @Obs.vis _ _ _ A₂ ev₂ k₂ =>
@@ -342,7 +344,7 @@ def eq {α} (it₁ it₂ : iTree E α) : Prop :=
   | _, .tau it₂ => eq it₁ it₂
   | _, _ => False
 coinductive_fixpoint monotonicity fun f f' himp => by
-  intro it₁ it₂ 
+  intro it₁ it₂
   match h : it₁.unfold with
   | .ret v₁ =>
     simp only [h]
@@ -369,7 +371,7 @@ coinductive_fixpoint monotonicity fun f f' himp => by
       rintro ⟨rfl, rfl, hk⟩
       refine ⟨rfl, ?_⟩
       refine ⟨.rfl, ?_⟩
-      intro a 
+      intro a
       specialize hk a
       apply himp
       exact hk
@@ -419,11 +421,11 @@ public def wb' (r : iTree E V → iTree E V → Prop) (it₁ it₂ : iTree E V) 
 def bisimulation : iTree E V → iTree E V → Prop := wb bisimulation
 coinductive_fixpoint monotonicity fun r r' himp => by
   intro it₁ it₂ H
-  induction H with 
+  induction H with
   | ret v =>  constructor
   | sync it₁ it₂ R =>
     constructor; apply himp; assumption
-  | vis ev k => 
+  | vis ev k =>
     constructor
     · assumption
     · intros; apply himp; grind only
@@ -445,7 +447,7 @@ end FirstTry
 namespace SecondTry
 
 public inductive wb (r : iTree E V → iTree E V → Prop) : iTree E V → iTree E V → Prop where
-| ret {it₁ it₂}  : ∀ v : V, 
+| ret {it₁ it₂}  : ∀ v : V,
     it₁.unfold = .ret v → it₂.unfold = .ret v →
     wb r it₁ it₂
 | vis  {it₁ it₂} : ∀ ev₁ k₁ ev₂ k₂,
@@ -458,22 +460,22 @@ public inductive wb (r : iTree E V → iTree E V → Prop) : iTree E V → iTree
     wb r it₁ it₂
 | tauL {it₁ it₂} : ∀ it₁',
     it₁.unfold = .tau it₁' →
-    wb r it₁' it₂ → 
+    wb r it₁' it₂ →
     wb r it₁ it₂
-| tauR {it₁ it₂} : ∀ it₂', 
+| tauR {it₁ it₂} : ∀ it₂',
     it₂.unfold = .tau it₂' →
     wb r it₁ it₂ → wb r it₁ it₂
 
 def eq : iTree E V → iTree E V → Prop := wb eq
 coinductive_fixpoint monotonicity fun r r' himp => by
   intro it₁ it₂ H
-  induction H with 
-  | ret v h₁ h₂ => 
+  induction H with
+  | ret v h₁ h₂ =>
     apply wb.ret v h₁ h₂
   | sync it₁ it₂ h₁ h₂ R =>
     apply wb.sync it₁ it₂ h₁ h₂
     apply himp; assumption
-  | vis ev₁ k₁ ev₂ k₂ h₁ h₂ hev IH => 
+  | vis ev₁ k₁ ev₂ k₂ h₁ h₂ hev IH =>
     apply wb.vis ev₁ k₁ ev₂ k₂ h₁ h₂ hev
     intros; apply himp; grind
   | tauL it₁' h₁ _ IH =>
@@ -487,6 +489,8 @@ coinductive_fixpoint monotonicity fun r r' himp => by
 end SecondTry
 
 namespace ThirdTry
+variable {E : Type quest → Type resp}{R : Type ret}
+
 
 /-
 
@@ -499,9 +503,8 @@ We define a weaker version of equality, observational
 -- in terms of one another.
 -- Might be useful for grind lemmas.
 
-mutual 
-  variable {R : Type _}{E : Type _ → Type _}
-
+mutual
+  -- Eqit (r : R → R → Prop) (l r : Bool) [i.e. eutt :0 Eqit (· = ·) true true]
   abbrev Rel (r : R → R → Prop) (it₁ it₂ : iTree E R)  : Prop := ObsRel r it₁.unfold it₂.unfold
   coinductive_fixpoint monotonicity by
     rintro Rel Rel' ⟨_, Obsimp⟩ it₁ it₂ H
@@ -509,29 +512,29 @@ mutual
     assumption
 
   def ObsRel (r : R → R → Prop) : Obs E R (iTree E R) → Obs E R (iTree E R) → Prop
-  | .ret v₁, .ret v₂ => 
+  | .ret v₁, .ret v₂ =>
       r v₁ v₂
   | .vis (A := A₁) ev₁ k₁, .vis (A := A₂) ev₂ k₂ =>
-      ∃ (h : A₁ = A₂), ev₁ = h ▸ ev₂ ∧ ∀ s₁, 
+      ∃ (h : A₁ = A₂), ev₁ = h ▸ ev₂ ∧ ∀ s₁,
         Rel r (k₁ s₁) (k₂ (h ▸ s₁))
   | .tau it₁', .tau it₂' =>
       Rel r it₁' it₂'
   | _, _ => False
   coinductive_fixpoint monotonicity by
     rintro ⟨Rel, Obs⟩ ⟨Rel', Obs'⟩ ⟨Rimp, _⟩ obs₁ obs₂ H
-    match h₁ : obs₁ with 
-    | .ret v₁ => 
+    match h₁ : obs₁ with
+    | .ret v₁ =>
         cases h₂ : obs₂ <;> grind
-    | .vis (A := A₁) ev₁ k₁ => 
-        match obs₂ with 
+    | .vis (A := A₁) ev₁ k₁ =>
+        match obs₂ with
         | .ret v₂ => grind
         | .tau it₂ => grind
-        | .vis (A := A₂) ev₂ k₂ => 
+        | .vis (A := A₂) ev₂ k₂ =>
           obtain ⟨h, rfl, ext⟩ := H
           simp only [Lean.Order.PartialOrder.rel, true_and, h, exists_true_left] at *
           intros; apply Rimp; apply ext
-    | .tau it₁ => 
-        match  obs₂ with 
+    | .tau it₁ =>
+        match  obs₂ with
         | .ret v₂ => grind
         | .vis (A := A₂) ev₂ k₂ => grind
         | .tau it₂ =>
@@ -541,56 +544,58 @@ mutual
 end
 
 
+--- lift (?). Maybe with `postFix`? ObsRelF? `eqitF` maybe
+-- coinduction template
 abbrev ObsRel.func (s : iTree E R → iTree E R → Prop) (r : R → R → Prop) : Obs E R (iTree E R) → Obs E R (iTree E R) → Prop
-| .ret v₁, .ret v₂ => 
+| .ret v₁, .ret v₂ =>
     r v₁ v₂
 | .vis (A := A₁) ev₁ k₁, .vis (A := A₂) ev₂ k₂ =>
-    ∃ (h : A₁ = A₂), ev₁ = h ▸ ev₂ ∧ ∀ s₁, 
+    ∃ (h : A₁ = A₂), ev₁ = h ▸ ev₂ ∧ ∀ s₁,
       s (k₁ s₁) (k₂ (h ▸ s₁))
 | .tau it₁', .tau it₂' =>
     s it₁' it₂'
 | _, _ => False
 
-/- def ObsRel (r : R → R → Prop)(it₁ it₂ : iTree E R) : Prop := -/ 
-/-   match it₁.unfold, it₂.unfold with -/ 
-/-   | .ret v₁, .ret v₂ => -/ 
+/- def ObsRel (r : R → R → Prop)(it₁ it₂ : iTree E R) : Prop := -/
+/-   match it₁.unfold, it₂.unfold with -/
+/-   | .ret v₁, .ret v₂ => -/
 /-       r v₁ v₂ -/
 /-   | .vis (A := A₁) ev₁ k₁, .vis (A := A₂) ev₂ k₂ => -/
-/-       ∃ (h : A₁ = A₂), ev₁ = h ▸ ev₂ ∧ ∀ s₁, -/ 
+/-       ∃ (h : A₁ = A₂), ev₁ = h ▸ ev₂ ∧ ∀ s₁, -/
 /-         ObsRel r (k₁ s₁) (k₂ (h ▸ s₁)) -/
 /-   | .tau it₁', .tau it₂' => -/
 /-       ObsRel r it₁' it₂' -/
 /-   | _, _ => False -/
 /- coinductive_fixpoint monotonicity fun ObsRel ObsRel' Himp it₁ it₂ H => by -/
-/-   dsimp at H ⊢ -/ 
-/-   match h₁ :  it₁.unfold with -/ 
-/-   | .ret v₁ => -/ 
-/-       simp [h₁] at H ⊢ -/ 
+/-   dsimp at H ⊢ -/
+/-   match h₁ :  it₁.unfold with -/
+/-   | .ret v₁ => -/
+/-       simp [h₁] at H ⊢ -/
 /-       cases h₂ : it₂.unfold <;> grind -/
-/-   | .vis (A := A₁) ev₁ k₁ => -/ 
-/-       simp [h₁] at H ⊢ -/ 
-/-       match h₂ : it₂.unfold with -/ 
+/-   | .vis (A := A₁) ev₁ k₁ => -/
+/-       simp [h₁] at H ⊢ -/
+/-       match h₂ : it₂.unfold with -/
 /-       | .ret v₂ => grind -/
 /-       | .tau it₂ => grind -/
-/-       | .vis (A := A₂) ev₂ k₂ => -/ 
-/-         simp [h₂] at H ⊢ -/ 
+/-       | .vis (A := A₂) ev₂ k₂ => -/
+/-         simp [h₂] at H ⊢ -/
 /-         obtain ⟨h, rfl, ext⟩ := H -/
 /-         subst h -/
-/-         simp -/ 
+/-         simp -/
 /-         intros -/
 /-         apply Himp -/
 /-         apply ext -/
-/-   | .tau it₁ => -/ 
-/-       simp [h₁] at H ⊢ -/ 
-/-       match h₂ : it₂.unfold with -/ 
+/-   | .tau it₁ => -/
+/-       simp [h₁] at H ⊢ -/
+/-       match h₂ : it₂.unfold with -/
 /-       | .ret v₂ => grind -/
 /-       | .vis (A := A₂) ev₂ k₂ => grind -/
 /-       | .tau it₂ => -/
-/-         simp [h₂] at H ⊢ -/ 
+/-         simp [h₂] at H ⊢ -/
 /-         apply Himp -/
 /-         assumption -/
 
-abbrev ObsEq{E R} (it₁ it₂ : iTree E R) := Rel (· = ·) it₁ it₂
+abbrev ObsEq (it₁ it₂ : iTree E R) := Rel (· = ·) it₁ it₂
 
 abbrev ObsEq.func s (obs₁ obs₂ : Obs E R (iTree E R)) := ObsRel.func s (·=·) obs₁ obs₂
 
@@ -601,10 +606,10 @@ instance {E : Type _ → Type _} : HasEquiv (iTree E R) where
 /- theorem ObsEq.cases (it₁ it₂ : iTree E R) : -/
 /-     it₁ ≈ it₂ → -/
 /-     (∃ v₁, it₁.unfold = .ret v₁) ∧ (∃ v₂, it₂.unfold = .ret v₂) ∨ -/
-/-     (∃ (A₁ : Type) (ev₁ : E A₁) (k₁ : A₁ → iTree E R), it₁.unfold = .vis ev₁ k₁) ∧ -/ 
+/-     (∃ (A₁ : Type) (ev₁ : E A₁) (k₁ : A₁ → iTree E R), it₁.unfold = .vis ev₁ k₁) ∧ -/
 /-     (∃ (A₂ : Type) (ev₂ : E A₂) (k₂ : A₂ → iTree E R), it₂.unfold = .vis ev₂ k₂) ∨ -/
 /-     (∃ it₁', it₁.unfold = .tau it₁') ∧ (∃ it₂', it₂.unfold = .tau it₂') := fun h => -/
-/-   match h₁ : it₁.unfold, h₂ : it₂.unfold with -/ 
+/-   match h₁ : it₁.unfold, h₂ : it₂.unfold with -/
 /-   | .ret v₁, .ret v₂ => by grind -/
 /-   | .vis (A := A₁) ev₁ k₁, .vis (A := A₂) ev₂ k₂ => by grind -/
 /-   | .tau it₁', .tau it₂' => by grind -/
@@ -617,7 +622,7 @@ instance {E : Type _ → Type _} : HasEquiv (iTree E R) where
 
 @[grind →]
 theorem ObsEq.obsEq_unfold_eq_ret {it₁ it₂ : iTree E R} :
-    it₁.unfold = .ret v₁ → 
+    it₁.unfold = .ret v₁ →
     it₁ ≈ it₂ →
     ∃ v₂, it₂.unfold = .ret v₂ := fun h₁ h => by
   unfold Rel at h
@@ -626,16 +631,16 @@ theorem ObsEq.obsEq_unfold_eq_ret {it₁ it₂ : iTree E R} :
 
 @[grind →]
 theorem ObsEq.obsEq_unfold_eq_vis {it₁ it₂ : iTree E R} {ev₁ : E A₁} {k₁} :
-    it₁.unfold = .vis ev₁ k₁ → 
+    it₁.unfold = .vis ev₁ k₁ →
     it₁ ≈ it₂ →
     ∃ (A₂ : Type _) (ev₂ : E A₂) (k₂ : A₂ → iTree E R), it₂.unfold = .vis ev₂ k₂ := fun h₁ h => by
   unfold Rel at h
   cases h₂ : it₂.unfold <;> simp [h₁, h₂, ObsRel] at h
   case vis A₂ ev₂ k₂ => exists A₂, ev₂, k₂
 
-@[grind →]
+@[grind →] -- Inversion lemmas (`_inv`)
 theorem ObsEq.obsEq_unfold_eq_tau {it₁ it₂ it₁' : iTree E R} :
-    it₁.unfold = .tau it₁' → 
+    it₁.unfold = .tau it₁' →
     it₁ ≈ it₂ →
     ∃ it₂', it₂.unfold = .tau it₂' := fun h₁ h => by
   unfold Rel at h
@@ -643,7 +648,7 @@ theorem ObsEq.obsEq_unfold_eq_tau {it₁ it₂ it₁' : iTree E R} :
   case tau it₂ => exists it₂
 
 theorem ObsEq.unfold_eq_ret {it₁ it₂ : iTree E R} {v₁ : R} {v₂ : R} :
-    it₁.unfold = .ret v₁ → 
+    it₁.unfold = .ret v₁ →
     it₂.unfold = .ret v₂ →
     it₁ ≈ it₂ →
     v₁ = v₂ := fun h₁ h₂ h => by
@@ -651,16 +656,16 @@ theorem ObsEq.unfold_eq_ret {it₁ it₂ : iTree E R} {v₁ : R} {v₂ : R} :
   simpa [h₁, h₂, ObsRel] using h
 
 theorem ObsEq.unfold_eq_vis {it₁ it₂ : iTree E R} {ev₁ : E A₁} {ev₂ : E A₂} {k₁ k₂} :
-    it₁.unfold = .vis ev₁ k₁ → 
+    it₁.unfold = .vis ev₁ k₁ →
     it₂.unfold = .vis ev₂ k₂ →
     it₁ ≈ it₂ →
-    ∃ (h : A₁ = A₂), ev₁ = h ▸ ev₂ ∧ ∀ s₁, 
+    ∃ (h : A₁ = A₂), ev₁ = h ▸ ev₂ ∧ ∀ s₁,
       (k₁ s₁) ≈ (k₂ (h ▸ s₁)) := fun h₁ h₂ h => by
   unfold Rel at h
   simpa [h₁, h₂, ObsRel] using h
 
 theorem ObsEq.unfold_eq_tau {it₁ it₂ it₁' : iTree E R} :
-    it₁.unfold = .tau it₁' → 
+    it₁.unfold = .tau it₁' →
     it₂.unfold = .tau it₂' →
     it₁ ≈ it₂ →
     it₁' ≈ it₂' := fun h₁ h₂ h => by
@@ -673,28 +678,33 @@ theorem ObsRel.iff_rel {it₁ it₂ : iTree E R} :
   unfold Rel
   exact ⟨id, id⟩
 
-    /- /1- set_option pp.all true in -1/ -/
+#check Rel.coinduct
+#print ObsRel.func
+
+-- parametrized coinduction (what rocq-paco does, actually)
 def ObsEq.coinductWith
-  (pred : iTree E R → iTree E R → Prop) 
-  {it₁ it₂ : iTree E R} 
+  (pred : iTree E R → iTree E R → Prop)
+  {it₁ it₂ : iTree E R}
   (baseCase : pred it₁ it₂)
   (progress :
     ∀ (it₁ it₂ : iTree E R),
-      pred it₁ it₂ → func pred it₁.unfold it₂.unfold) :
+      pred it₁ it₂ → ObsEq.func pred it₁.unfold it₂.unfold) :
     ObsEq it₁ it₂ := by
   apply Rel.coinduct (·=·) (pred_1 := pred) (pred_2 := ObsEq.func pred) _ _ _ _ baseCase
   all_goals grind only
 
-theorem ObsEq.refl (it : iTree E R) : it ≈ it := by 
+@[refl]
+theorem ObsEq.refl {it : iTree E R} : it ≈ it := by
   apply ObsEq.coinductWith (·=·) rfl
   grind only
- 
-theorem ObsEq.symm (it₁ it₂ : iTree E R) : it₁ ≈ it₂ → it₂ ≈ it₁ := by 
+
+ @[symm]
+theorem ObsEq.symm {it₁ it₂ : iTree E R} : it₁ ≈ it₂ → it₂ ≈ it₁ := by
   intro h
-  apply ObsEq.coinductWith (pred := fun x y => y ≈ x) h 
+  apply ObsEq.coinductWith (pred := fun x y => y ≈ x) h
   intros it₁ it₂ hyp
-  match h₁ : it₁.unfold, h₂ : it₂.unfold with 
-  | Obs.ret _, Obs.ret _ => 
+  match h₁ : it₁.unfold, h₂ : it₂.unfold with
+  | Obs.ret _, Obs.ret _ =>
     grind [ObsEq.unfold_eq_ret]
   | Obs.vis (A := A₁) ev₁ k₁, Obs.vis (A := A₂) ev₂ k₂ =>
     grind [ObsEq.unfold_eq_vis]
@@ -705,16 +715,16 @@ theorem ObsEq.symm (it₁ it₂ : iTree E R) : it₁ ≈ it₂ → it₂ ≈ it�
   | .vis .., .ret ..
   | .vis .., .tau ..
   | .tau .., .vis ..
-  | .tau .., .ret .. => 
+  | .tau .., .ret .. =>
     unfold Rel at hyp
     simp [h₁, h₂,  ObsRel] at hyp
 
-theorem ObsEq.trans (it₁ it₂ it₃ : iTree E R) : it₁ ≈ it₂ → it₂ ≈ it₃ → it₁ ≈ it₃ := by 
+theorem ObsEq.trans {it₁ it₂ it₃ : iTree E R} : it₁ ≈ it₂ → it₂ ≈ it₃ → it₁ ≈ it₃ := by
   intro it12 it23
   apply ObsEq.coinductWith (pred := fun x z => ∃ y, x ≈ y ∧ y ≈ z) ⟨it₂, it12, it23⟩
   rintro it₁ it₃ ⟨it₂, it12, it23⟩
-  match h₁ : it₁.unfold, h₃ : it₃.unfold with 
-  | Obs.ret _, Obs.ret _ => 
+  match h₁ : it₁.unfold, h₃ : it₃.unfold with
+  | Obs.ret _, Obs.ret _ =>
     grind [ObsEq.unfold_eq_ret]
   | Obs.vis (A := A₁) ev₁ k₁, Obs.vis (A := A₃) ev₃ k₃ =>
     grind [ObsEq.unfold_eq_vis]
@@ -729,26 +739,26 @@ theorem ObsEq.trans (it₁ it₂ it₃ : iTree E R) : it₁ ≈ it₂ → it₂ 
   | .vis .., .ret ..
   | .vis .., .tau ..
   | .tau .., .vis ..
-  | .tau .., .ret .. => 
+  | .tau .., .ret .. =>
     have oit12 := ObsRel.iff_rel.1 it12
     have oit23 := ObsRel.iff_rel.1 it23
     grind
 
-instance : Std.Refl (@ObsEq E R) where refl := ObsEq.refl
-instance : Std.Symm (@ObsEq E R) where symm := ObsEq.symm
-instance : Trans (@ObsEq E R) (@ObsEq E R) (@ObsEq E R) where trans := ObsEq.trans _ _ _
+instance : Std.Refl (@ObsEq E R) where refl _ := ObsEq.refl
+instance : Std.Symm (@ObsEq E R) where symm _ _ := ObsEq.symm
+instance : Trans (@ObsEq E R) (@ObsEq E R) (@ObsEq E R) where trans := ObsEq.trans
 
-def ObsEq.step_tau_obsEq_self (it : iTree E R) (s : it.State) c : 
+def ObsEq.step_tau_obsEq_self (it : iTree E R) (s : it.State) c :
     { {it with curr := c}.tau with curr := .inr s } ≈ {it with curr := s} := by
-  apply ObsEq.coinductWith (fun 
-    (iTree.mk (State := State₁) curr₁ step₁) 
+  apply ObsEq.coinductWith (fun
+    (iTree.mk (State := State₁) curr₁ step₁)
     (iTree.mk (State := State₂) curr₂ step₂) =>
-    ∃ (H : State₁ = (Unit ⊕ State₂)),
+    ∃ (H : State₁ = (PUnit ⊕ State₂)),
     curr₁ = H.mpr (Sum.inr curr₂) ∧
-    ∀ (s : State₂), 
+    ∀ (s : State₂),
     step₁ (H ▸ (.inr s)) = H.symm ▸ (step₂ s).mapState .inr
   )
-  case baseCase => 
+  case baseCase =>
     simp [tau, Obs.mapState]
   case progress =>
     unfold func ObsRel.func unfold
@@ -757,41 +767,43 @@ def ObsEq.step_tau_obsEq_self (it : iTree E R) (s : it.State) c :
     cases _ : s₂ c₂ <;>
     simp [*, Obs.mapState]
 
-def ObsEq.step_vis_obsEq_self {E R A} (it : iTree E R) (ev : E A) (kS : A → it.State) (a : A) :
+def ObsEq.step_vis_obsEq_self (it : iTree E R) (ev : E A) (kS : A → it.State) (a : A) :
     { curr := kS a, step := it.step : iTree E R} ≈
     { curr : Unit ⊕ (_ : A) × it.State := Sum.inr ⟨a, kS a⟩,
         step := fun x =>
           match x with
           | Sum.inl PUnit.unit => Obs.vis ev fun a => Sum.inr ⟨a, kS a⟩
           | Sum.inr ⟨a, s⟩ => Obs.mapState (fun x => Sum.inr ⟨a, x⟩) (it.step s) } := by
-  apply ObsEq.coinductWith (fun 
-    (iTree.mk (State := State₁) curr₁ step₁) 
+  apply ObsEq.coinductWith (fun
+    (iTree.mk (State := State₁) curr₁ step₁)
     (iTree.mk (State := State₂) curr₂ step₂) =>
-    ∃ (H : State₂ = (Unit ⊕ (_ : A) × State₁)),
-    curr₂ = H.mpr (Sum.inr ⟨a, curr₁⟩) ∧
-    ∀ (s : State₁), 
-    step₂ (H ▸ (.inr ⟨a, s⟩)) = H.symm ▸ (step₁ s).mapState (.inr ⟨a, ·⟩)
+    ∃ (mpr : (PUnit ⊕ (_ : A) × State₁) → State₂),
+    curr₂ = mpr (Sum.inr ⟨a, curr₁⟩) ∧
+    ∀ (s : State₁),
+    step₂ (mpr (.inr ⟨a, s⟩)) = (step₁ s).mapState (mpr <| .inr ⟨a, ·⟩)
   )
-  case baseCase => 
+  case baseCase =>
+    exists id
     simp [Obs.mapState]
   case progress =>
-    rintro ⟨c₁, s₁⟩ ⟨c₂, s₂⟩ ⟨rfl, HC, Hs⟩
+    rintro ⟨c₁, s₁⟩ ⟨c₂, s₂⟩ ⟨h, HC, Hs⟩
     unfold ObsEq.func ObsRel.func unfold
     cases _ : s₁ c₁ <;>
     cases _ : s₂ c₂ <;>
     simp [*, Obs.mapState]
+    all_goals (intros; exists h)
 
-/- def ObsEq.step_vis_obsEq_self {E : Type _ → Type _}(ev : E A) (k : A → S) (a : A) (s : S) c : -/ 
+/- def ObsEq.step_vis_obsEq_self {E : Type _ → Type _}(ev : E A) (k : A → S) (a : A) (s : S) c : -/
     /- { iTree.vis ev (fun a => ⟨c, k a⟩) with curr := .inr ⟨a, s⟩ } ≈ {it with curr := s} := by -/
-  /- apply ObsEq.coinductWith (fun -/ 
-  /-   (iTree.mk (State := State₁) curr₁ step₁) -/ 
+  /- apply ObsEq.coinductWith (fun -/
+  /-   (iTree.mk (State := State₁) curr₁ step₁) -/
   /-   (iTree.mk (State := State₂) curr₂ step₂) => -/
   /-   ∃ (H : State₁ = (Unit ⊕ State₂)), -/
   /-   curr₁ = H.mpr (Sum.inr curr₂) ∧ -/
-  /-   ∀ (s : State₂), -/ 
+  /-   ∀ (s : State₂), -/
   /-   step₁ (H ▸ (.inr s)) = H.symm ▸ (step₂ s).mapState .inr -/
   /- ) -/
-  /- case baseCase => -/ 
+  /- case baseCase => -/
   /-   simp [tau, Obs.mapState] -/
   /- case progress => -/
   /-   unfold func ObsRel.func unfold -/
@@ -826,7 +838,19 @@ theorem ObsEq.obsEq_tau_of_unfold_tau {it it': iTree E R} : it.unfold = .tau it'
     have := step_tau_obsEq_self it st st |>.symm
     simpa [tau, h]
 
-set_option pp.universes true in
+theorem ObsEq.obsEq_tau_of_obsEq_unfold_tau {it it'₁ it'₂ : iTree E R} :
+    it.unfold = .tau it'₁ →
+    it'₁ ≈ it'₂ →
+    it ≈ .tau it'₂ := by
+  simp [unfold]
+  cases h : it.step it.curr <;> simp
+  case tau st =>
+  rintro rfl heq
+  have := ObsEq.tau_congr heq
+  refine ObsEq.trans ?_ this
+  unfold Rel ObsRel unfold
+  simpa [*, tau] using ObsEq.step_tau_obsEq_self it st st |>.symm
+
 theorem ObsEq.obsEq_vis_of_unfold_vis {it : iTree E R}{ev : E A} {k}: it.unfold = .vis ev k → it ≈ .vis ev k := by
   simp [unfold]
   cases h : it.step it.curr <;> simp
@@ -840,95 +864,233 @@ theorem ObsEq.obsEq_vis_of_unfold_vis {it : iTree E R}{ev : E A} {k}: it.unfold 
     /- assumption -/
     -- TODO: Idk why I can't conclude with the previous, so I just copy-paste the proof
     -- of `ObsEq.step_vis_obsEq_self`
-    apply ObsEq.coinductWith (fun 
-      (iTree.mk (State := State₁) curr₁ step₁) 
+    apply ObsEq.coinductWith (fun
+      (iTree.mk (State := State₁) curr₁ step₁)
       (iTree.mk (State := State₂) curr₂ step₂) =>
-      ∃ (H : State₂ = (Unit ⊕ (_ : A) × State₁)),
-      curr₂ = H.mpr (Sum.inr ⟨a, curr₁⟩) ∧
-      ∀ (s : State₁), 
-      step₂ (H ▸ (.inr ⟨a, s⟩)) = H.symm ▸ (step₁ s).mapState (.inr ⟨a, ·⟩)
+      ∃ (mpr : PUnit ⊕ (_ : A) × State₁ → State₂),
+      curr₂ = mpr (Sum.inr ⟨a, curr₁⟩) ∧
+      ∀ (s : State₁),
+      step₂ (mpr (.inr ⟨a, s⟩)) = (step₁ s).mapState (mpr <| .inr ⟨a, ·⟩)
     )
-    case baseCase => 
+    case baseCase =>
+      exists id
       simp [Obs.mapState]
     case progress =>
-      rintro ⟨c₁, s₁⟩ ⟨c₂, s₂⟩ ⟨rfl, HC, Hs⟩
+      rintro ⟨c₁, s₁⟩ ⟨c₂, s₂⟩ ⟨h, HC, Hs⟩
       unfold ObsEq.func ObsRel.func unfold
       cases _ : s₁ c₁ <;>
       cases _ : s₂ c₂ <;>
       simp [*, Obs.mapState]
+      all_goals (intros; exists h)
 
-instance instEquiv {E R} : Equivalence (fun (x y : iTree E R) => x ≈ y) where
-  refl :=  ObsEq.refl
-  symm := ObsEq.symm _ _
-  trans := ObsEq.trans _ _ _
+theorem ObsEq.unfold_vis (ev : E A) (k : A → iTree E R) :
+    ObsRel (·=·) (iTree.vis ev k).unfold (Obs.vis ev k) := by
+  simp [unfold, iTree.vis, ObsRel]
+  intro a
+  apply ObsEq.coinductWith (fun
+    (iTree.mk (State := State₂) curr₂ step₂)
+    (iTree.mk (State := State₁) curr₁ step₁) =>
+    ∃ (mpr : (Unit ⊕ (_ : A) × State₁) → State₂),
+    curr₂ = mpr (Sum.inr ⟨a, curr₁⟩) ∧
+    ∀ (s : State₁),
+    step₂ (mpr (.inr ⟨a, s⟩)) = (step₁ s).mapState (mpr <| .inr ⟨a, ·⟩)
+  )
+  case baseCase =>
+    simp
+    exists (fun | .inl .unit => .inl .unit
+                | .inr ⟨_, st⟩ => .inr ⟨a, st⟩ )
+    simp [Obs.mapState]
+  case progress =>
+    rintro ⟨c₁, s₁⟩ ⟨c₂, s₂⟩ ⟨h, HC, Hs⟩-- ⟨h, HC, Hs⟩
+    unfold ObsEq.func ObsRel.func unfold
+    cases h₁ : s₁ c₁ <;>
+    cases h₂ : s₂ c₂ <;>
+    simp [*, Obs.mapState]
+    all_goals (intros; exists h)
 
-instance instSetoid.{a,e,r} {E : Type a → Type e}{R : Type r}: Setoid (iTree.{a,e,r} E R) where
-  r := (· ≈ ·)
+
+def iTree.obsEqElim {motive : iTree E R → Type _}
+  (inv : ∀ {it it'}, it ≈ it' → motive it' → motive it)
+  (ret : ∀ (v : R), motive (.ret v))
+  (vis : ∀ (A : Type _) (ev : E A) (k : A → iTree E R), motive (.vis ev k))
+  (tau : ∀ (it : iTree E R), motive (.tau it)) :
+    ∀ it, motive it := fun it => by
+  match h : it.unfold with
+  | .ret v =>
+    exact inv (ObsEq.obsEq_ret_of_unfold_ret h) (ret ..)
+  | .tau it' =>
+    exact inv (ObsEq.obsEq_tau_of_unfold_tau h) (tau ..)
+  | .vis ev k =>
+    exact inv (ObsEq.obsEq_vis_of_unfold_vis h) (vis ..)
+
+instance instEquiv  : Equivalence (fun (x y : iTree E R) => x ≈ y) where
+  refl  := Std.Refl.refl
+  symm  := Std.Symm.symm _ _
+  trans := Trans.trans
+
+instance instSetoid : Setoid (iTree E R) where
+  r := ObsEq
   iseqv := instEquiv
 
 def iTree'.{a,e,r} (E : Type a → Type e) (R : Type r) : Type _ := Quotient (instSetoid (E := E) (R := R))
 
-set_option pp.universes true in #print iTree'
+#check Quotient.mk
+#check Quotient.lift
+#check Quotient.sound
 
-def iTree'.mk {E : Type _ → Type _} {R : Type _}(it : iTree E R)  := Quotient.mk inferInstance it
+namespace iTree'
 
-def iTree'.unfold (it' : iTree' E R) : Obs E R (iTree' E R) := 
+def mk (it : iTree E R)  := Quotient.mk instSetoid it
+
+def unfold (it' : iTree' E R) : Obs E R (iTree' E R) :=
   it'.lift (fun it =>
-    match it.unfold with 
-    | Obs.ret v => Obs.ret v
-    | Obs.tau it₂ => Obs.tau (iTree'.mk it₂)
-    | Obs.vis ev k => 
-      Obs.vis ev (fun a => iTree'.mk (k a))
-  ) (by 
+    it.unfold.mapState iTree'.mk
+  ) (by
     intros it₁ it₂ heq
     match h₁ : it₁.unfold, h₂ : it₂.unfold with
-    | Obs.ret _, Obs.ret _ => 
+    | Obs.ret _, Obs.ret _ =>
       simp [h₁, h₂]
       grind only [ObsEq.unfold_eq_ret]
     | Obs.vis (A := A₁) ev₁ k₁, Obs.vis (A := A₂) ev₂ k₂ =>
-      simp [*]
+      simp [*, Obs.mapState]
       obtain ⟨rfl, rfl, ih⟩:= ObsEq.unfold_eq_vis h₁ h₂ heq
       simp only [heq_eq_eq, true_and]
-      ext 
+      ext
       apply Quotient.sound
       apply ih
     | Obs.tau it₁', Obs.tau it₃' =>
-      simp [*]
+      simp [*, Obs.mapState]
       apply Quotient.sound
       apply ObsEq.unfold_eq_tau h₁ h₂ heq
-      /- grind [ObsEq.unfold_eq_tau] -/
     | .ret .., .tau ..
     | .ret .., .vis ..
     | .vis .., .ret ..
     | .vis .., .tau ..
     | .tau .., .vis ..
-    | .tau .., .ret .. => 
+    | .tau .., .ret .. =>
       grind)
 
-def iTree'.out (it' : iTree' E R) : iTree E R where
+def out (it' : iTree' E R) : iTree E R where
     curr := it'
     step := iTree'.unfold
-    
-def iTree'.ret {R : Type _} (v : R){E : Type _ → Type _} := iTree'.mk (.ret v : iTree E R)
 
-def iTree'.tau {R : Type _} {E : Type _ → Type _} (it : iTree' E R) := 
-    it.lift (Quotient.mk inferInstance <| iTree.tau ·) (by 
+theorem unfold_out (it' : iTree' E R) :
+    ObsRel (·=·) (it'.unfold.mapState (·.out)) (it'.out.unfold) :=
+  -- Basically, we can unfold either in the quotient our outside of it
+    sorry
+/-   apply it'.ind -/
+/-   intros it -/
+/-   cases h: it.unfold <;> -/
+/-   simp [h, unfold, Quotient.lift, Quotient.mk, out, Obs.mapState] -/
+/-   sorry -/
+
+def ret {R : Type _} (v : R){E : Type _ → Type _} := iTree'.mk (.ret v : iTree E R)
+
+theorem unfold_eq_ret (v : R) (it' : iTree' E R) :
+    it'.unfold = .ret v → it' = iTree'.ret v := by
+  apply it'.ind; intro it
+  intros h
+  simp [ret]
+  apply Quotient.sound
+  apply ObsEq.obsEq_ret_of_unfold_ret
+  simp [unfold, Quotient.lift, Quotient.mk, Obs.mapState] at h
+  cases h₂ : it.unfold <;> simp [h₂] at h
+  simpa
+
+def tau {R : Type _} {E : Type _ → Type _} (it : iTree' E R) :=
+    it.lift (Quotient.mk inferInstance <| iTree.tau ·) (by
       intros it it' heq; simp; apply Quotient.sound
       apply ObsEq.tau_congr heq
     )
 
-def iTree'.vis {A : Type a} {R : Type _}{E : Type a → Type _} (ev : E A) (k' : A → iTree' E R) : iTree' E R := 
-  let k := fun a => (k' a).out
-  iTree'.mk (.vis ev k)
+theorem unfold_eq_tau (it' it'₂ : iTree' E R) :
+    it'.unfold = .tau it'₂ →
+    it' = iTree'.tau it'₂ := by
+  apply it'.ind; intros it
+  apply it'₂.ind; intro it₂
+  intros h
+  simp [tau, Quotient.lift, Quotient.mk]
+  apply Quotient.sound
+  simp [unfold, Quotient.lift, Quotient.mk, Obs.mapState] at h
+  cases h₂ : it.unfold <;> simp [h₂] at h
+  case a.tau it₂ =>
+    have h := Quotient.exact h
+    apply ObsEq.obsEq_tau_of_obsEq_unfold_tau h₂ h
 
-set_option pp.universes true in #print iTree'
+-- def vis {A : Type a} {R : Type _}{E : Type a → Type _} (ev : E A) (k' : A → iTree' E R) : iTree' E R :=
+--   let k := fun a =>
+--     (k' a).out
+--   iTree'.mk (.vis ev k)
 
-def iTree'.cases.{r,a,e,s} {R : Type r}{E : Type a → Type e} {motive : iTree'.{a,e,r,s} E R → Type _} 
+-- /- set_option pp.universes true in -/
+-- -- TODO: The issue here is that we're comparing things at different universe levels.
+-- -- In a sense, this is allowing us to `shrink` the universes.
+-- theorem unfold_eq_vis (it' : iTree'.{quest,resp,ret,s} E R) (ev : E A) (k' : A → iTree'.{quest,resp,ret,s} E R) :
+--     it'.unfold = .vis ev k' →
+--     it' = iTree'.vis ev k'
+--     := by
+--   apply it'.ind; intros it
+--   intros h
+--   simp [tau, Quotient.lift, Quotient.mk]
+--   apply Quotient.sound
+--   simp [unfold, Quotient.lift, Quotient.mk, Obs.mapState] at h
+--   cases h₂ : it.unfold <;> simp [h₂] at h
+--   case a.tau it₂ =>
+--     have h := Quotient.exact h
+--     apply ObsEq.obsEq_tau_of_obsEq_unfold_tau h₂ h
+
+instance piSetoid {ι : Sort _} {α : ι → Sort _} [∀ i, Setoid (α i)] : Setoid (∀ i, α i) where
+  r a b := ∀ i, a i ≈ b i
+  iseqv := ⟨fun _ _ ↦ Setoid.refl _,
+            fun h _ ↦ Setoid.symm (h _),
+            fun h₁ h₂ _ ↦ Setoid.trans (h₁ _) (h₂ _)⟩
+
+unsafe def _root_.Quot.unquot {r : α → α → Prop} : Quot r → α :=
+  cast lcProof
+
+unsafe
+def Quotient.bubbleUpUnsafe {X A : Type _}{s : Setoid X}(f : A → Quotient s) : Quotient (piSetoid : Setoid (A → X)) :=
+  .mk (_) (fun i ↦ (f i).unquot)
+
+noncomputable def _root_.Quot.out {r : α → α → Prop} (q : Quot r) : α :=
+  Classical.choose (Quot.exists_rep q)
+
+noncomputable def _root_.Quotient.choice {ι : Type _} {α : ι → Type _} {S : ∀ i, Setoid (α i)}
+    (f : ∀ i, Quotient (S i)) :
+    @Quotient (∀ i, α i) (by infer_instance) :=
+  .mk _ (fun i ↦ (f i).out)
+
+@[implemented_by Quotient.bubbleUpUnsafe]
+noncomputable
+def _root_.Quotient.bubbleUp{X A : Type _}{s : Setoid X}(f : A → Quotient s) : Quotient (piSetoid : Setoid (A → X)) :=
+  Quotient.choice (ι := A) (α := λ_↦X) (S := λ_↦s) f
+
+
+
+def vis {A : Type a} {R : Type _}{E : Type a → Type _} (ev : E A) (k' : A → iTree' E R) : iTree' E R :=
+  (Quotient.bubbleUp k').lift (.mk <| iTree.vis ev ·) (
+    fun k₁ k₂ k₁k₂ =>
+    Quotient.sound <| by
+    change ObsEq (iTree.vis ev k₁) (iTree.vis ev k₂)
+    unfold ObsEq Rel
+    have h₁ := ObsEq.unfold_vis ev k₁
+    have h₂ := ObsEq.unfold_vis ev k₂
+    have : ObsRel (·=·) (Obs.vis ev k₁) (Obs.vis ev k₂) := by
+      unfold ObsRel
+      exists rfl
+    sorry -- TODO: Put it all together, may need to define symm and trans for `ObsRel`.
+  )
+
+
+
+def elim {R : Type r}{E : Type a → Type e} {motive : iTree' E R → Type _}
   (ret : (v : R) → motive (.ret v))
   (vis : ∀ {A : Type a} (ev : E A) (k : A → iTree' E R), motive (iTree'.vis ev k))
-  (tau : (it : iTree' E R) → motive (.tau it)) : 
-    ∀ (it' : iTree' E R), motive it' := by
+  (tau : (it : iTree' E R) → motive (.tau it)) :
+    ∀ (it' : iTree' E R), motive it' := fun it => by
   sorry
+
+end iTree'
 
 end ThirdTry
 
@@ -946,13 +1108,13 @@ instance : HasEquiv (iTree E R) where Equiv := SecondTry.eq
 /-   intros h -/
 /-   unfold bindLeft -/
 /-   sorry -/
-  
 
-theorem id_map {α : Type} (it : iTree E α) : bindLeft pure it ≈ it := by 
+
+theorem id_map {α : Type} (it : iTree E α) : bindLeft pure it ≈ it := by
   dsimp [HasEquiv.Equiv]
   unfold eq
-  match h : it.unfold with 
-  | .ret v₁ => 
+  match h : it.unfold with
+  | .ret v₁ =>
     cases h₂ : it.step it.curr <;> (try simp [h₂, unfold] at h; done)
     apply wb.tauL ?_ ?unfold ?next
     case unfold =>
@@ -962,7 +1124,7 @@ theorem id_map {α : Type} (it : iTree E α) : bindLeft pure it ≈ it := by
     simp [unfold, pure, ret]
     simp [unfold, h₂] at h
     assumption
-  | .vis ev₁ k₁ => 
+  | .vis ev₁ k₁ =>
     cases h₂ : it.step it.curr <;> (try simp [h₂, unfold] at h; done)
     case vis A ev₁ k₁ =>
     /- have := h -/
@@ -977,17 +1139,17 @@ theorem id_map {α : Type} (it : iTree E α) : bindLeft pure it ≈ it := by
       simp [unfold, h₂, pure, ret]
       sorry
     all_goals sorry
-  | .tau it₁ => 
+  | .tau it₁ =>
     sorry
 
 instance  : LawfulMonad (iTree E) := .mk'
-   (id_map     := by 
+   (id_map     := by
       simp only [Functor.map, bind, Pure.pure, Function.comp_id]
       intros α it
       have {State, curr, step} := it
       simp [bindLeft, *]
       sorry
-      /- induction it <;> simp [bindLeft, *] -/ 
+      /- induction it <;> simp [bindLeft, *] -/
     )
    (pure_bind  := by intros α β it f; simp only [bind, bindLeft])
    (bind_assoc := by intros α β γ it f g; simp only [bind]; induction it <;> simp [bindLeft, *])
